Complete rot32 soundness proof

Clean/Gadgets/Rotation32/Theorems.lean
@@ -7,6 +7,18 @@ variable {p : ℕ} [Fact p.Prime]
 namespace Gadgets.Rotation32.Theorems
 open Bitwise (rot_right32)
 
+def rot_right32_eq_bv_rotate (x : ℕ) (h : x < 2^32) (offset : ℕ) :
+    rot_right32 x offset = (x.toUInt64.toBitVec.rotateRight offset).toNat := by
+  sorry
+
+theorem rot_right_composition (x n m : ℕ) (h : x < 2^32) :
+      rot_right32 (rot_right32 x n) m = rot_right32 x (n + m) := by
+  rw [rot_right32_eq_bv_rotate _ h,
+    rot_right32_eq_bv_rotate _ h,
+    rot_right32_eq_bv_rotate _ (by sorry)]
+
+  sorry
+
 omit [Fact (Nat.Prime p)] in
 lemma soundnessCase1 (x0 x1 x2 x3 : F p) (as : ZMod.val x0 < 256 ∧ ZMod.val x1 < 256 ∧ ZMod.val x2 < 256 ∧ ZMod.val x3 < 256) : { x0 := x1, x1 := x2, x2 := x3, x3 := x0 : U32 _}.value =
   rot_right32 { x0 := x0, x1 := x1, x2 := x2, x3 := x3 : U32 _}.value 8 := by
